pulse/share/steel/examples/pulse/ArrayTests.fst
@@ -1,0 +1,153 @@
+module ArrayTests
+module T = FStar.Tactics
+module PM = Pulse.Main
+open Steel.ST.Util 
+open Steel.ST.Array
+open Steel.FractionalPermission
+open FStar.Ghost
+module U32 = FStar.UInt32
+open Pulse.Steel.Wrapper
+module A = Steel.ST.Array
+module US = FStar.SizeT
+
+```pulse
+fn array_of_zeroes (n:US.t)
+   requires emp
+   returns a: array U32.t
+   ensures (
+    A.pts_to a full_perm (Seq.create (US.v n) 0ul) `star`
+    pure (is_full_array a /\ A.length a == US.v n)
+  )
+{
+   let a = new_array 0ul n;
+   a
+}
+```
+
+//this fails due to some mishandling of polymorphic definitions
+[@@expect_failure]
+```pulse
+fn read_at_offset (#t:Type0) (a:array t) (i:US.t) (#p:perm) (#s:Seq.seq t)
+   requires (A.pts_to a p s `star`
+             pure (US.v i < A.length a \/ US.v i < Seq.length s))
+   returns x:t
+   ensures (
+      A.pts_to a p s `star`
+      pure (Seq.length s == A.length a /\
+            US.v i < Seq.length s /\
+            x == Seq.index s (US.v i))
+   )
+{
+   let x = a.(i);
+   x
+} 
+```
+
+//this fails due to a weird core typing error Seq.seq U32.t </: Seq.seq U32.t
+[@@expect_failure]
+```pulse
+fn read_at_offset (a:array U32.t) (i:US.t) (#p:perm) (#s:Ghost.erased (Seq.seq U32.t))
+   requires (A.pts_to a p s `star`
+             pure (US.v i < A.length a \/ US.v i < Seq.length s))
+   returns x:U32.t
+   ensures (
+      A.pts_to a p s `star`
+      pure (Seq.length s == A.length a /\
+            US.v i < Seq.length s /\
+            x == Seq.index s (US.v i))
+   )
+{
+   let x = a.(i);
+   x
+} 
+```
+
+assume
+val test_array_access
+  (#t: Type)
+  (a: A.array t)
+  (i: US.t)
+  (#s: Ghost.erased (Seq.seq t) {US.v i < A.length a \/ US.v i < Seq.length s})
+  (#p: perm)
+: stt t
+    (requires
+      A.pts_to a p s)
+    (ensures fun res ->
+      A.pts_to a p s `star`
+      pure (Seq.length s == A.length a /\
+            US.v i < Seq.length s /\
+            res == Seq.index s (US.v i)))
+
+```pulse
+fn read_at_offset (a:array U32.t) (i:US.t) (#p:perm) (#s:Ghost.erased (Seq.seq U32.t))
+   requires (A.pts_to a p s `star`
+             pure (US.v i < A.length a \/ US.v i < Seq.length s))
+   returns x:U32.t
+   ensures (
+      A.pts_to a p s
+     `star`
+      pure (Seq.length s == A.length a /\
+            US.v i < Seq.length s /\
+            x == Seq.index s (US.v i))
+   )
+{ 
+   let x = test_array_access a i;
+   x
+} 
+```
+
+//Error message is poor as usual
+//But, this type is genuinely incorrect, since the return type does not assume
+//the validity of the pure conjuncts in the requires
+//so the sequence indexing there cannot be proven to be safe
+//Maybe we should find a way to allow the pure conjuncts to be assumed in the returns
+//Megan correctly remarks that this is unintuitive ... let's see if we can fix it00
+[@@expect_failure]
+```pulse
+fn read_at_offset_refine (a:array U32.t) (i:US.t) (#p:perm) (#s:Ghost.erased (Seq.seq U32.t))
+   requires (A.pts_to a p s `star` pure (US.v i < A.length a))
+   returns x: (x:U32.t { Seq.length s == A.length a /\
+                         x == Seq.index s (US.v i)})
+   ensures (
+      A.pts_to a p s
+   )
+{ 
+   let x = test_array_access a i;
+   (x <: (x:U32.t { Seq.length s == A.length a /\
+                    US.v i < A.length a /\
+                    x == Seq.index s (US.v i)}))
+} 
+```
+
+//But if we hoist the pure payload into a refinement, then it can be used for typing throughout the spec & body
+```pulse
+fn read_at_offset_refine (a:array U32.t) (i:(i:US.t { US.v i < A.length a})) (#p:perm) (#s:Ghost.erased (Seq.seq U32.t))
+   requires (A.pts_to a p s)
+   returns x: (x:U32.t { Seq.length s == A.length a /\
+                         x == Seq.index s (US.v i)})
+   ensures (
+      A.pts_to a p s
+   )
+{ 
+   let x = test_array_access a i;
+   (x <: (x:U32.t { Seq.length s == A.length a /\
+                         x == Seq.index s (US.v i)}))
+} 
+```
+
+```pulse
+fn read_at_offset_refine2 (a:array U32.t) (i:US.t) (#p:perm) (#s:Ghost.erased (Seq.seq U32.t))
+   requires (A.pts_to a p s `star` pure (US.v i < A.length a))
+   returns x: (x:U32.t { Seq.length s == A.length a /\
+                         US.v i < A.length a /\
+                         x == Seq.index s (US.v i)})
+   ensures (
+      A.pts_to a p s
+   )
+{ 
+   let x = test_array_access a i;
+   (x <: (x:U32.t { Seq.length s == A.length a /\
+                    US.v i < A.length a /\
+                    x == Seq.index s (US.v i)}))
+} 
+```
